after a bunch of experimentation, settled on a slightly modified version of Gensyn_Sem that I feel reasonably good about. Now trying to sort out locale issues...

Semantics/Gensyn_Semantics.thy
@@ -10,6 +10,7 @@ datatype ('x) gs_result =
   | GRPath childpath
   | GRCrash
   | GRDone
+  | GRFuel
   | GROther 'x
 
 type_synonym gensyn_skel = "(unit, unit, unit) gensyn"
@@ -20,7 +21,7 @@ inductive nosem_base_sem::
     'mstate \<Rightarrow> 
     'mstate \<Rightarrow> 
       childpath \<Rightarrow>
-      gensyn_skel \<Rightarrow>  
+      ('b, 'r, 'g) gensyn \<Rightarrow>  
       ('rxb) gs_result \<Rightarrow>
       bool"
   where  "nosem_base_sem _ _ _ _ _ _ GRUnhandled"
@@ -44,7 +45,7 @@ inductive nosem_rec_sem ::
     'mstate \<Rightarrow> 
     'mstate \<Rightarrow> 
       childpath \<Rightarrow>
-      gensyn_skel \<Rightarrow>  
+      ('b, 'r, 'g) gensyn \<Rightarrow>  
       ('rxr) gs_result \<Rightarrow>
       bool"
   where "nosem_rec_sem _ _ _ _ _ _ GRUnhandled"
@@ -119,8 +120,8 @@ fixes rec_result_sem :: "'result \<Rightarrow>
                       'mstate \<Rightarrow> 
                       'mstate \<Rightarrow> 
                       childpath \<Rightarrow>
-                      gensyn_skel \<Rightarrow>  
-                      ('bxr) gs_result \<Rightarrow>
+                      ('b, 'r, 'g) gensyn \<Rightarrow>  
+                      ('xr) gs_result \<Rightarrow>
                       bool"
 
   fixes rec_sem :: "'g \<Rightarrow>
@@ -128,8 +129,8 @@ fixes rec_result_sem :: "'result \<Rightarrow>
                     'mstate \<Rightarrow>
                     'mstate \<Rightarrow>
                     childpath \<Rightarrow>
-                    gensyn_skel \<Rightarrow>
-                    ('rxr) gs_result \<Rightarrow>
+                    ('b, 'r, 'g) gensyn \<Rightarrow>
+                    ('xr) gs_result \<Rightarrow>
                     bool"
 
 (* question: dealing with state abstraciton.
@@ -155,23 +156,23 @@ inductive gensyn_sem ::
   where
   "\<And> t cp g b m m' .
     gensyn_get t cp = Some (GBase g b) \<Longrightarrow>
-    base_sem g b m m' cp (gs_strip t) GRDone \<Longrightarrow>
+    base_sem g b m m' cp t GRDone \<Longrightarrow>
     gensyn_sem t cp m m'"
 
 | "\<And> t cp g b m cp' m' m'' .
     gensyn_get t cp = Some (GBase g b) \<Longrightarrow>
-    base_sem g b m m' cp (gs_strip t) (GRPath cp') \<Longrightarrow>
+    base_sem g b m m' cp t (GRPath cp') \<Longrightarrow>
     gensyn_sem t cp' m' m'' \<Longrightarrow>
     gensyn_sem t cp m m''"
 
 | "\<And> t cp g r l m m' .
    gensyn_get t cp = Some (GRec g r l) \<Longrightarrow>
-   rec_sem g r m m' cp (gs_strip t) GRDone \<Longrightarrow>
+   rec_sem g r m m' cp t GRDone \<Longrightarrow>
    gensyn_sem t cp m m'"
 
 | "\<And> t cp g r l m cp' m' m'' .
    gensyn_get t cp = Some (GRec g r l) \<Longrightarrow>
-   rec_sem g r m m' cp (gs_strip t) (GRPath cp') \<Longrightarrow>
+   rec_sem g r m m' cp t (GRPath cp') \<Longrightarrow>
    gensyn_sem t cp' m' m'' \<Longrightarrow>
    gensyn_sem t cp m m''"
 
@@ -180,22 +181,66 @@ end
 interpretation Gensyn_Semantics_Nosem : Gensyn_Semantics
   nosem_base_sem nosem_rec_sem
   done
-(*
+
+(* i don't know if these are actually useful *)
+fun unskel :: "(gensyn_skel \<Rightarrow> ('a, 'b, 'c) gensyn)" where
+"unskel (GBase () ()) = GBase undefined undefined"
+| "unskel (GRec () () l) = GRec undefined undefined (map unskel l)"
+  
+fun skel_lift1 :: "(('a, 'b, 'c) gensyn \<Rightarrow> bool) \<Rightarrow> gensyn_skel \<Rightarrow> bool"
+  where
+"skel_lift1 p s = p (unskel s)"
+
+fun skel_lift2 :: "(gensyn_skel \<Rightarrow> bool) \<Rightarrow> ('a, 'b, 'c) gensyn \<Rightarrow> bool" where
+"skel_lift2 p s = p (gs_strip s)"
+
+(* test - numnodes predicate *)
+fun gensyn_numnodes :: "('a, 'b, 'c) gensyn \<Rightarrow> nat" and
+    gensyn_numnodes_l :: "('a, 'b, 'c) gensyn list \<Rightarrow> nat" where
+"gensyn_numnodes (GBase _ _) = 1"
+| "gensyn_numnodes (GRec _ _ l) = 1 + gensyn_numnodes_l l"
+| "gensyn_numnodes_l [] = 1"
+| "gensyn_numnodes_l (h#t) = gensyn_numnodes h + gensyn_numnodes_l t"
+
+lemma gensyn_numnodes_l_nz : "gensyn_numnodes_l l > (0 :: nat)"
+proof(induction l)
+  case Nil
+  then show ?case by auto
+next
+  case (Cons a l)
+  then show ?case 
+    apply(case_tac a, auto)
+    done
+qed
+
+fun gensyn_two_nodes :: "('a, 'b, 'c) gensyn \<Rightarrow> bool" where
+ "gensyn_two_nodes g = (gensyn_numnodes g = 2)"
+
+lemma preds_equal :
+    "skel_lift1 gensyn_two_nodes (GRec ()() [])"
+  apply(simp)
+  done
+
+(* in order to characterize when this works, though, we are going to
+   need a way to characterize what the predicate is actually looking at *)
+
 locale Gensym_Semantics_Exec =
-  fixes base_sem_exec :: "('b, 'r, 'g) gensyn \<Rightarrow>
+  fixes base_sem_exec :: "
                       'g \<Rightarrow> 
                       'b \<Rightarrow> 
+                      'mstate \<Rightarrow>
                       childpath \<Rightarrow> 
-                      'mstate \<Rightarrow> 
-                      (childpath option *
+                      ('b, 'r, 'g) gensyn \<Rightarrow> 
+                      ('xr gs_result *
                       'mstate) option"
 
-  fixes rec_sem_exec :: "('b, 'r, 'g) gensyn \<Rightarrow>
+  fixes rec_sem_exec :: "
                       'g \<Rightarrow>
                       'r \<Rightarrow>
-                      childpath \<Rightarrow>
                       'mstate \<Rightarrow>
-                      (childpath option *
+                      childpath \<Rightarrow>
+                      ('b, 'r, 'g) gensyn \<Rightarrow>
+                      ('xr gs_result *
                       'mstate) option"
 
 begin
@@ -217,15 +262,17 @@ fun gensyn_sem_exec ::
     (case gensyn_get t cp of
      None \<Rightarrow> None
      | Some (GBase g b) \<Rightarrow>
-       (case base_sem_exec t g b cp m of
+       (case base_sem_exec g b m cp t of
              None \<Rightarrow> None
-             | Some (None, m') \<Rightarrow> Some m'
-             | Some (Some cp', m') \<Rightarrow> gensyn_sem_exec t cp' m' n)
+             | Some (GRDone, m') \<Rightarrow> Some m'
+             | Some (GRPath cp', m') \<Rightarrow> gensyn_sem_exec t cp' m' n
+             | Some (_, _) \<Rightarrow> None)
      | Some (GRec g r l) \<Rightarrow>
-        (case rec_sem_exec t g r cp m of
+        (case rec_sem_exec g r m cp t of
              None \<Rightarrow> None
-             | Some (None, m') \<Rightarrow> Some m'
-             | Some (Some cp', m') \<Rightarrow> gensyn_sem_exec t cp' m' n))"
+             | Some (GRDone, m') \<Rightarrow> Some m'
+             | Some (GRPath cp', m') \<Rightarrow> gensyn_sem_exec t cp' m' n
+             | Some (_, _) \<Rightarrow> None))"
 
 lemma gensyn_sem_exec_morefuel :
   assumes H: "gensyn_sem_exec t cp m n = Some m'"
@@ -246,78 +293,70 @@ next
     proof(cases a)
       case (GBase x11 x12)
       then show ?thesis using Suc Some
-      proof(cases "base_sem_exec t x11 x12 cp m")
-        assume None': "base_sem_exec t x11 x12 cp m = None"
+      proof(cases "base_sem_exec x11 x12 m cp t")
+        assume None': "base_sem_exec x11 x12 m cp t = None"
         then show ?thesis using Suc Some GBase by auto
       next
         fix stm'
-        assume Some': "base_sem_exec t x11 x12 cp m = Some stm'"
+        assume Some': "base_sem_exec x11 x12 m cp t = Some stm'"
         then show ?thesis
         proof(cases stm')
           case (Pair st' m'')
-          then show ?thesis
-          proof(cases st')
-            assume None'' : "st' = None"
-            thus ?thesis using Pair Some' GBase Some Suc by auto
-          next
-            fix st's
-            assume Some'' : "st' = Some st's"
-            thus ?thesis using Pair Some' GBase Some Suc by auto
-          qed
+          then show ?thesis using Pair Some' GBase Some Suc
+            apply(case_tac st', auto)
+            done
         qed
       qed
     next
       case (GRec x21 x22 x23)
       then show ?thesis
-      proof(cases "rec_sem_exec t x21 x22 cp m")
-        assume None' :"rec_sem_exec t x21 x22 cp m = None"
+      proof(cases "rec_sem_exec x21 x22 m cp t")
+        assume None' :"rec_sem_exec x21 x22 m cp t = None"
         then show ?thesis using Suc Some GRec by auto
       next
         fix stm'
-        assume Some': "rec_sem_exec t x21 x22 cp m = Some stm'"
+        assume Some': "rec_sem_exec x21 x22 m cp t = Some stm'"
         then show ?thesis
         proof(cases stm')
           case (Pair st' m'')
-          then show ?thesis
-          proof(cases st')
-            assume None'' : "st' = None"
-            thus ?thesis using Pair Some' GRec Some Suc by auto
-          next
-            fix st's
-            assume Some'' : "st' = Some st's"
-            thus ?thesis using Pair Some' GRec Some Suc by auto
-          qed
+          then show ?thesis using Pair Some' GRec Some Suc
+            apply(case_tac st', auto)
+            done
         qed
       qed
     qed
   qed
 qed
 
-definition gsx_base_sem :: "('b, 'r, 'g) gensyn \<Rightarrow>
-                      'g \<Rightarrow> 
+fun gsx_base_sem :: " 'g \<Rightarrow> 
                       'b \<Rightarrow> 
+                      'mstate \<Rightarrow>
+                      'mstate \<Rightarrow>
                       childpath \<Rightarrow> 
-                      'mstate \<Rightarrow> 
-                      childpath option \<Rightarrow>
-                      'mstate \<Rightarrow> 
+                      ('b, 'r, 'g) gensyn \<Rightarrow>
+                      ('xr) gs_result \<Rightarrow>
                       bool"
   where
-"gsx_base_sem  =
-  (\<lambda> t g b cp m cp' m' . base_sem_exec t g b cp m = Some (cp', m'))"
+"gsx_base_sem g b m m' cp t res = 
+    (case base_sem_exec g b m cp t of
+        None \<Rightarrow> m' = m \<and> res = GRFuel
+        | Some (res', m'') \<Rightarrow> m' = m'' \<and> res = res')"
 
-definition gsx_rec_sem :: "('b, 'r, 'g) gensyn \<Rightarrow>
-                    'g \<Rightarrow>
+fun gsx_rec_sem :: "'g \<Rightarrow>
                     'r \<Rightarrow>
+                    'mstate \<Rightarrow>
+                    'mstate \<Rightarrow>
                     childpath \<Rightarrow>
-                    'mstate \<Rightarrow>
-                    childpath option \<Rightarrow>
-                    'mstate \<Rightarrow>
+                    ('b, 'r, 'g) gensyn \<Rightarrow>
+                    ('xr) gs_result \<Rightarrow>
                     bool"
   where
-"gsx_rec_sem  =
-  (\<lambda>  t g r cp m cp' m' . rec_sem_exec t g r cp m = Some (cp', m'))"
+"gsx_rec_sem g r m m' cp t res =
+  (case rec_sem_exec g r m cp t of
+    None \<Rightarrow> m' = m \<and> res = GRFuel
+    | Some (res', m'') \<Rightarrow> m' = m'' \<and> res = res')"
 
-definition gsx_gensyn_sem ::
+fun gsx_gensyn_sem ::
 "('b, 'r, 'g) gensyn \<Rightarrow>
    childpath \<Rightarrow>
    'mstate \<Rightarrow>
@@ -325,48 +364,51 @@ definition gsx_gensyn_sem ::
    bool
   "
 where
-"gsx_gensyn_sem  =
-  (\<lambda> t cp m m' . \<exists> fuel . gensyn_sem_exec t cp m fuel = Some m')"
-(*
+"gsx_gensyn_sem t cp m m' =  (\<exists> fuel . gensyn_sem_exec t cp m fuel = Some m')"
+
 (* standard version of the semantics *)
-interpretation Gensym_Exec_Semantics : Gensym_Semantics
+interpretation Gensyn_Exec_Semantics : Gensyn_Semantics
  gsx_base_sem gsx_rec_sem
   done
 
 lemma gensyn_exec_eq_l2r :
   fixes t cp m m'
-  shows  "Gensym_Exec_Semantics.gensyn_sem t cp m m' \<Longrightarrow> gsx_gensyn_sem t cp m m'"
-  proof(induction rule: Gensym_Exec_Semantics.gensyn_sem.induct)
+  shows  "Gensyn_Exec_Semantics.gensyn_sem t cp m m' \<Longrightarrow> gsx_gensyn_sem t cp m m'"
+  proof(induction rule: Gensyn_Exec_Semantics.gensyn_sem.induct)
 case (1 t cp g b m m')
   then show ?case
-    apply(simp add: gsx_gensyn_sem_def gsx_base_sem_def)
+    apply(simp)
     apply(rule_tac x = 1 in exI) apply(auto)
+    apply(case_tac "base_sem_exec g b m cp t", auto)
     done
 next
 case (2 t cp g b m cp' m' m'')
   then show ?case
-    apply(simp add: gsx_gensyn_sem_def gsx_base_sem_def)
+    apply(simp)
     apply(auto)
     apply(rule_tac x = "Suc fuel" in exI) apply(auto)
+    apply(case_tac "base_sem_exec g b m cp t", auto)
     done
 next
   case (3 t cp g r l m m')
   then show ?case
-    apply(simp add: gsx_gensyn_sem_def gsx_rec_sem_def)
+    apply(simp)
     apply(rule_tac x = 1 in exI) apply(auto)
+    apply(case_tac "rec_sem_exec g r m cp t", auto)
     done
 next
   case (4 t cp g r l m cp' m' m'')
   then show ?case
-    apply(simp add: gsx_gensyn_sem_def gsx_rec_sem_def)
+    apply(simp)
     apply(auto)
     apply(rule_tac x = "Suc fuel" in exI) apply(auto)
+    apply(case_tac "rec_sem_exec g r m cp t", auto)
     done
 qed
 
 lemma gensyn_exec_eq_r2l :
   fixes fuel
-  shows "\<And> t cp m m'. gensyn_sem_exec t cp m (fuel) = Some m' \<Longrightarrow> Gensym_Exec_Semantics.gensyn_sem t cp m m'"
+  shows "\<And> t cp m m'. gensyn_sem_exec t cp m (fuel) = Some m' \<Longrightarrow> Gensyn_Exec_Semantics.gensyn_sem t cp m m'"
   proof(induction fuel)
     case 0
     then show ?case by auto
@@ -381,81 +423,58 @@ lemma gensyn_exec_eq_r2l :
       then show ?thesis using Suc
       proof(cases a)
         case (GBase x11 x12) then show ?thesis using Some Suc
-        proof(cases "base_sem_exec t x11 x12 cp m")
-          assume None' : "base_sem_exec t x11 x12 cp m = None"
+        proof(cases "base_sem_exec x11 x12 m cp t")
+          assume None' : "base_sem_exec x11 x12 m cp t = None"
           thus ?thesis using GBase Some Suc by auto
         next
           fix a'
-          assume Some' : "base_sem_exec t x11 x12 cp m = Some a'"
+          assume Some' : "base_sem_exec x11 x12 m cp t = Some a'"
           thus ?thesis using GBase Some Suc
           proof(cases a')
             case (Pair a'' b)
             then show ?thesis using Some' GBase Some Suc
-            proof(cases a'')
-              assume None'' : "a'' = None"
-              then show ?thesis using Pair Some' GBase Some Suc Gensym_Semantics.gensyn_sem.intros
-                by (auto simp add:gsx_base_sem_def)
-            next
-              fix a'''
-              assume Some'' : "a'' = Some a'''"
-              then show ?thesis using Pair Some' GBase Some Suc 
-                    Gensym_Semantics.gensyn_sem.intros(2)[of t cp x11 x12 gsx_base_sem]
-                by (auto simp add:gsx_base_sem_def)
-            qed
+              apply(simp)
+              apply(case_tac a'', auto simp add: Gensyn_Semantics.gensyn_sem.intros)
+              done
           qed
         qed
       next
-
-  case (GRec x21 x22 x23)
-  then show ?thesis using Some Suc
-  proof(cases "rec_sem_exec t x21 x22 cp m")
-    assume None' : "rec_sem_exec t x21 x22 cp m = None"
-    thus ?thesis using GRec Some Suc by auto
-  next
-
-    fix a'
-    assume Some' : "rec_sem_exec t x21 x22 cp m = Some a'"
-    thus ?thesis using GRec Some Suc
-    proof(cases a')
-      case (Pair a'' b)
-      then show ?thesis
-      proof(cases a'')
-        assume None'' : "a'' = None"
-        thus ?thesis using GRec Some Suc Some' Pair
-              Gensym_Semantics.gensyn_sem.intros gsx_rec_sem_def
-          by auto
-
-      next
-
-        fix a'''
-        assume Some'' : "a'' = Some a'''"
-        thus ?thesis using GRec Some Suc Some' Pair
-              Gensym_Semantics.gensyn_sem.intros(4)[of t cp x21 x22 x23 gsx_rec_sem] gsx_rec_sem_def
-          by auto
+        case (GRec x21 x22 x23)
+        then show ?thesis using Some Suc
+          proof(cases "rec_sem_exec x21 x22 m cp t")
+            assume None' : "rec_sem_exec x21 x22 m cp t = None"
+            thus ?thesis using GRec Some Suc by auto
+          next
+        fix a'
+        assume Some' : "rec_sem_exec x21 x22 m cp t = Some a'"
+        thus ?thesis using GRec Some Suc
+        proof(cases a')
+          case (Pair a'' b)
+            then show ?thesis using Some' GRec Some Suc
+              apply(simp)
+              apply(case_tac a'', auto simp add: Gensyn_Semantics.gensyn_sem.intros)
+              done
+          qed
+        qed
       qed
     qed
-  qed
 qed
-qed
-qed
-*)
-(* version of the semantics that just wraps the fueled interpreter *)
-(* OK, we need some kind of lemma that will let us turn (f = g) into (forall x, f x = g x) *)
-interpretation Gensym_Exec_Semantics_Fuel : Gensym_Semantics
+
+
+interpretation Gensyn_Exec_Semantics_Fuel : Gensyn_Semantics
  gsx_base_sem gsx_rec_sem
- rewrites Crew : "Gensym_Exec_Semantics.gensyn_sem = gsx_gensyn_sem"
+ rewrites Crew : "Gensyn_Exec_Semantics.gensyn_sem = gsx_gensyn_sem"
 proof(unfold_locales)
-  have Goal : "\<And> t cp m m' . Gensym_Exec_Semantics.gensyn_sem t cp m m' = gsx_gensyn_sem t cp m m'" 
+  have Goal : "\<And> t cp m m' . Gensyn_Exec_Semantics.gensyn_sem t cp m m' = gsx_gensyn_sem t cp m m'" 
   proof - 
     fix t cp m m'
-    show "Gensym_Exec_Semantics.gensyn_sem t cp m m' = gsx_gensyn_sem t cp m m'"
+    show "Gensyn_Exec_Semantics.gensyn_sem t cp m m' = gsx_gensyn_sem t cp m m'"
       using gensyn_exec_eq_l2r
-                             gensyn_exec_eq_r2l gsx_gensyn_sem_def by auto
+                             gensyn_exec_eq_r2l  by auto
   qed
 
-    thus "Gensym_Exec_Semantics.gensyn_sem = gsx_gensyn_sem" by blast
+    thus "Gensyn_Exec_Semantics.gensyn_sem = gsx_gensyn_sem" by blast
   qed
 
-end
-*)
+
 end
